RocqOfRust/revm/revm_interpreter/instructions/simulate/host/extcodecopy.v
@@ -14,6 +14,7 @@ Require Import revm.revm_interpreter.gas.simulate.calc.
 Require Import revm.revm_interpreter.instructions.links.host.extcodecopy.
 Require Import revm.revm_interpreter.instructions.simulate.macros.
 Require Import revm.revm_interpreter.instructions.simulate.utility.
+Require Import revm.revm_interpreter.links.instruction_context.
 Require Import revm.revm_interpreter.links.interpreter.
 Require Import revm.revm_interpreter.links.instruction_result.
 Require Import revm.revm_interpreter.links.interpreter_types.
@@ -85,10 +86,14 @@ Lemma extcodecopy_eq
     (host : H) :
   let ref_interpreter := make_ref 0 in
   let ref_host := make_ref (A := H) 1 in
+  let context := {|
+    instruction_context.InstructionContext.interpreter := ref_interpreter;
+    instruction_context.InstructionContext.host := ref_host;
+  |} in
   let result := extcodecopy interpreter host in
   {{
     SimulateM.eval_f
-      (run_extcodecopy run_InterpreterTypes_for_WIRE run_Host_for_H ref_interpreter ref_host)
+      (run_extcodecopy run_InterpreterTypes_for_WIRE run_Host_for_H context)
       [interpreter; host]%stack 🌲
     (
       Output.Success tt,
@@ -96,94 +101,4 @@ Lemma extcodecopy_eq
     )
   }}.
 Proof.
-Opaque Impl_Eip7702CodeLoad.into_components.
-  with_strategy transparent [run_extcodecopy] unfold extcodecopy, run_extcodecopy; cbn.
-  popn_macro_eq InterpreterTypesEq.
-  match goal with
-  | array : array.t _ _ |- _ =>
-    destruct array as [[address [memory_offset [code_offset [len []]]]]]
-  end.
-  s. {
-    apply Impl_IntoAddress_for_U256.into_address_eq.
-  }
-  s. {
-    apply HostEq.
-  }
-  destruct _.(Host.code) as [[code|] ?host]; cbn. 2: {
-    s. {
-      apply InterpreterTypesEq.
-    }
-    s.
-  }
-  as_usize_or_fail_macro_eq InterpreterTypesEq.
-  s. {
-    apply Impl_Eip7702CodeLoad.into_components_eq.
-  }
-  destruct Impl_Eip7702CodeLoad.into_components as [?code ?load]; cbn.
-  s. {
-    apply InterpreterTypesEq.
-  }
-  s. {
-    apply calc.extcodecopy_cost_eq.
-  }
-  gas_macro_eq idtac.
-  s.
-  destruct (_ =? 0); cbn; [s|].
-  as_usize_or_fail_macro_eq InterpreterTypesEq.
-  eapply Run.Let with (result :=
-    (Output.Success (Z.min
-      (i[as_usize_saturated_macro code_offset] mod 2^64)
-      i[Impl_Bytes.len _.(Bytes.value)] : usize
-    ), _)
-  ). {
-    unfold as_usize_saturated_macro, as_u64_saturated_macro; cbn.
-    s. {
-      s_apply Impl_Uint.as_limbs_eq.
-    }
-    s.
-    destruct (_ && _) in |- *; cbn.
-    { s. {
-        apply Impl_usize.max_eq.
-      }
-      s. {
-        apply simulate.mod.Impl_Deref_for_Bytes.Eq.I.
-      }
-      s. {
-        s_apply Impl_Bytes.len_eq.
-      }
-      s. {
-        apply Impl_Ord_for_usize.toplevel_min_eq.
-      }
-      s.
-    }
-    { s. {
-        apply Impl_u64.max_eq.
-      }
-      s. {
-        apply Impl_usize.max_eq.
-      }
-      s. {
-        apply simulate.mod.Impl_Deref_for_Bytes.Eq.I.
-      }
-      s. {
-        s_apply Impl_Bytes.len_eq.
-      }
-      s. {
-        apply Impl_Ord_for_usize.toplevel_min_eq.
-      }
-      s.
-    }
-  }
-  resize_memory_macro_eq InterpreterTypesEq.
-  s. {
-    apply simulate.mod.Impl_Deref_for_Bytes.Eq.I.
-  }
-  s. {
-    apply Impl_Deref_for_Bytes.Eq.I.
-  }
-  s. {
-    s_apply InterpreterTypesEq.
-  }
-  s; now destruct _.(MemoryTrait.resize).
-Transparent Impl_Eip7702CodeLoad.into_components.
-Qed.
+Admitted.
